Fp/SmtLibSemantics.lean
@@ -389,7 +389,6 @@ theorem smtLibRoundMethod.tieBreak_eq {R : Type} (e s : Nat)
     (v.embed (v.lower r) < ves.embed (ves.lower r)) =
     (ves.embed (ves.upper r) < (v.embed (v.upper r)))) := rfl
 
-@[simp]
 theorem smtLibRoundMethod.roundForSign_eq {R : Type} (e s : Nat)
     (v : RoundableAdjunction (PackedFloat e s) R)
     (ves : RoundableAdjunction (PackedFloat e (s + 1)) R)
