Fp/Theorems/LowerUpperRound/Basic.lean
@@ -1,0 +1,539 @@
+import Fp.UnpackedRound
+import Fp.SmtLibSemantics
+import Fp.Theorems.SmtLibSemanticsQ
+import Fp.Theorems.PackedFloat.Packing
+import Fp.Theorems.PackedFloat.Negation
+import Fp.Theorems.PackedFloat.Ordering
+
+namespace Fp
+
+@[elab_as_elim]
+theorem PackedFloat.kindCasesNaNInfZeroNum {P : PackedFloat e s → Prop}
+    (x : PackedFloat e s)
+    (nanCase : ∀ (n : PackedFloat e s), n.isNaN → P n)
+    (infCase : ∀ sign, P (PackedFloat.getInfinity e s sign))
+    (zeroCase : ∀ sign, P (PackedFloat.getZero e s sign))
+    (numCase : ∀ (n : PackedFloat e s), n.isNormOrNonzeroSubnorm → P n) :
+    P x := by
+  have := x.classification_exhaustive
+  simp at this
+  by_cases h1 : x.isNaN
+  · grind
+  · by_cases h2 : x.isInfinite
+    · grind
+    · by_cases h3 : x.isZero
+      · grind
+      · by_cases h4 : x.isNonzeroSubnorm
+        · grind
+        · by_cases h5 : x.isNorm
+          · grind
+          · grind
+
+
+@[simp]
+theorem roundQ_eq (eout sout : Nat) (rm : RoundingMode) (sign : Bool) (r : ExtRat):
+    (Fp.SmtLibSemanticsQ.smtLibRoundMethodQ eout sout).round rm sign r =
+    (SmtLibSemantics.smtLibRoundMethod eout sout
+      SmtLibSemantics.smtLibV SmtLibSemantics.smtLibV).round rm sign
+    r := rfl
+
+@[simp]
+theorem isNaN_of_isLawfulLower (x : PackedFloat e s)
+   (hlower : SmtLibSemantics.IsLawfulLower ExtRat.NaN x) :
+    x.isNaN := by
+  simp [SmtLibSemantics.IsLawfulLower] at hlower
+  simp [hlower]
+
+@[simp]
+theorem isLawfulLower_of_isNaN :
+  (SmtLibSemantics.IsLawfulLower ExtRat.NaN (PackedFloat.getNaN e s)) := by
+  simp only [SmtLibSemantics.IsLawfulLower]
+  simp only [SmtLibSemantics.smtLibV_embed_eq, PackedFloat.toExtRat_eq_toExtRat',
+    PackedFloat.isNaN_getNaN, PackedFloat.toExtRat'_eq_NaN_of_isNaN, ExtRat.ge_eq_le_symm,
+    ExtRat.ExtRat.le_NaN_iff, decide_true, PackedFloat.toExtRat'_eq_NaN_iff_isNaN,
+    Bool.decide_eq_true, PackedFloat.le_iff_eq_of_isNaN', imp_self, implies_true, and_self]
+
+@[simp]
+theorem isLawfulLower_NaN_iff_isNaN (x : PackedFloat e s) :
+   SmtLibSemantics.IsLawfulLower ExtRat.NaN x ↔ x.isNaN := by
+  simp only [SmtLibSemantics.IsLawfulLower, SmtLibSemantics.smtLibV_embed_eq,
+    PackedFloat.toExtRat_eq_toExtRat', ExtRat.ge_eq_le_symm, ExtRat.ExtRat.le_NaN_iff,
+    PackedFloat.toExtRat'_eq_NaN_iff_isNaN, Bool.decide_eq_true, and_iff_left_iff_imp]
+  intros hx
+  intros lower hlower
+  simp [hx, hlower]
+
+@[elab_as_elim]
+theorem Classical.epsilon_elim {α : Sort u} {p q : α → Prop} (y : α) (hy : p y)
+   (hpq : ∀ x, p x → q x) :
+    q (@Classical.epsilon α (Nonempty.intro y) p) := by
+  apply hpq
+  apply Classical.epsilon_spec_aux
+  · exists y
+
+
+
+@[simp]
+theorem IsLawfulUpper_NaN_mkNaN :
+   SmtLibSemantics.IsLawfulUpper ExtRat.NaN (PackedFloat.getNaN e s) := by
+  simp [SmtLibSemantics.IsLawfulUpper]
+
+@[simp]
+theorem isLawfulUpper_NaN_iff_isNaN (x : PackedFloat e s) :
+   SmtLibSemantics.IsLawfulUpper ExtRat.NaN x ↔ x.isNaN := by
+  simp only [SmtLibSemantics.IsLawfulUpper, SmtLibSemantics.smtLibV_embed_eq,
+    PackedFloat.toExtRat_eq_toExtRat', ExtRat.ge_eq_le_symm, ExtRat.ExtRat.NaN_le_iff,
+    PackedFloat.toExtRat'_eq_NaN_iff_isNaN, Bool.decide_eq_true, and_iff_left_iff_imp]
+  intros hx upper
+  simp [hx]
+
+@[simp]
+theorem isNaN_upper_NaN :
+  (SmtLibSemantics.smtLibUpper.upper ExtRat.NaN : PackedFloat e s).isNaN := by
+  simp only [SmtLibSemantics.smtLibUpper, isLawfulUpper_NaN_iff_isNaN]
+  apply Classical.epsilon_elim (q := fun (x : PackedFloat e s) => x.isNaN) (y := PackedFloat.getNaN e s)
+  · simp
+  · simp
+
+@[simp]
+theorem isNaN_lower_NaN (e s : Nat) :
+    (SmtLibSemantics.smtLibLower.lower ExtRat.NaN : PackedFloat e s).isNaN := by
+  simp [SmtLibSemantics.smtLibLower]
+  apply Classical.epsilon_elim (q := fun (x : PackedFloat e s) => x.isNaN) (y := PackedFloat.getNaN e s)
+  · simp
+  · intros x hx
+    simp [hx]
+
+
+@[simp]
+theorem roundRNA_mkNaN (eout sout : Nat) (sign : Bool) :
+  ((SmtLibSemantics.smtLibRoundMethod eout sout SmtLibSemantics.smtLibV SmtLibSemantics.smtLibV).roundRNA sign
+    (ExtRat.NaN)).isNaN := by
+  simp [SmtLibSemantics.RoundMethod.roundRNA]
+
+@[simp]
+theorem roundRNE_mkNaN (eout sout : Nat) (sign : Bool) :
+   ((SmtLibSemantics.smtLibRoundMethod eout sout SmtLibSemantics.smtLibV SmtLibSemantics.smtLibV).roundRNE sign
+    (ExtRat.NaN)).isNaN := by
+  simp [SmtLibSemantics.RoundMethod.roundRNE, SmtLibSemantics.ExtendedNumber.isNaN]
+
+@[simp]
+theorem roundRTP_mkNaN (eout sout : Nat) (sign : Bool) :
+   ((SmtLibSemantics.smtLibRoundMethod eout sout SmtLibSemantics.smtLibV SmtLibSemantics.smtLibV).roundRTP sign
+    (ExtRat.NaN)).isNaN := by
+  simp [SmtLibSemantics.RoundMethod.roundRTP]
+
+
+
+@[simp]
+theorem roundRTN_mkNaN (eout sout : Nat) (sign : Bool) :
+  ((SmtLibSemantics.smtLibRoundMethod eout sout SmtLibSemantics.smtLibV SmtLibSemantics.smtLibV).roundRTN sign
+    (ExtRat.NaN)).isNaN := by
+  simp [SmtLibSemantics.RoundMethod.roundRTN]
+
+
+@[simp]
+theorem roundRTZ_mkNaN {eout sout : Nat} {sign : Bool} :
+  ((SmtLibSemantics.smtLibRoundMethod eout sout SmtLibSemantics.smtLibV SmtLibSemantics.smtLibV).roundRTZ sign
+    (ExtRat.NaN)).isNaN := by
+  simp [SmtLibSemantics.RoundMethod.roundRTZ, SmtLibSemantics.ExtendedNumber.isZero, ExtRat.eq,
+    SmtLibSemantics.ExtendedNumber.gtZero, SmtLibSemantics.ExtendedNumber.smtLibEq,
+    SmtLibSemantics.ExtendedNumber.ltZero]
+
+@[simp]
+theorem isNaN_round_of_nan {sign} {eout sout : Nat} {rm : RoundingMode} :
+    ((SmtLibSemantics.smtLibRoundMethod eout sout SmtLibSemantics.smtLibV SmtLibSemantics.smtLibV).round
+        rm sign ExtRat.NaN).isNaN := by
+  rcases rm <;> simp
+
+
+@[simp]
+theorem IsLawfulLower_Zero_iff (x : PackedFloat e s) (he : 0 < e) :
+   SmtLibSemantics.IsLawfulLower (ExtRat.Number 0) x ↔ (x = PackedFloat.getZero e s false) := by
+  simp [SmtLibSemantics.IsLawfulLower]
+  constructor
+  · intros h
+    obtain ⟨h1, h2⟩ := h
+    specialize h2 (PackedFloat.getZero e s false)
+    simp [PackedFloat.isZero_getZero, he, decide_true,
+      Bool.not_eq_true, forall_const] at h2
+    specialize (h2 (by grind))
+    by_cases hzero : x.isZero
+    · simp [hzero] at h1
+      simp [h1] at h2
+      grind only [PackedFloat.eq_mkZero_of_isZero']
+    · simp [hzero] at h1
+      grind only
+  · intros h
+    simp [h]
+    simp [he]
+    constructor
+    · grind
+    · intros lower hlower
+      by_cases hzero : lower.isZero
+      · simp [hzero]
+        have hlower : lower = PackedFloat.getZero e s lower.sign := by
+          grind only [PackedFloat.eq_mkZero_of_isZero']
+        rw [hlower]
+        simp [he]
+      · simp [hzero]
+        intros hsign
+        apply PackedFloat.le_of_sign_eq_true_sign_eq_false
+        · grind
+        · grind
+        · grind
+        · grind
+
+@[simp]
+theorem lower_zero_eq {eout sout : Nat} (heout : 0 < eout)  :
+  (SmtLibSemantics.smtLibLower.lower (ExtRat.Number 0) : PackedFloat eout sout) =
+    PackedFloat.getZero eout sout false := by
+  simp [SmtLibSemantics.smtLibLower]
+  apply Classical.epsilon_elim (q := fun (x : PackedFloat eout sout) => x = PackedFloat.getZero eout sout false)
+    (y := PackedFloat.getZero eout sout false)
+  · rw [IsLawfulLower_Zero_iff]
+    · grind
+  · intros x hx
+    simp [IsLawfulLower_Zero_iff, heout] at hx
+    simp [hx]
+
+-- TODO: Can we somehow unify the lower/upper proofs?
+@[simp]
+theorem IsLawfulUpper_Zero_iff (x : PackedFloat e s) (he : 0 < e) :
+   SmtLibSemantics.IsLawfulUpper (ExtRat.Number 0) x ↔ ((x = PackedFloat.getZero e s true)):= by
+  simp [SmtLibSemantics.IsLawfulUpper]
+  constructor
+  · intros h
+    obtain ⟨h1, h2⟩ := h
+    specialize h2 (PackedFloat.getZero e s true)
+    simp [PackedFloat.isZero_getZero, he, decide_true,
+      Bool.not_eq_true, forall_const] at h2
+    specialize (h2 (by grind))
+    by_cases hzero : x.isZero
+    · simp [hzero] at h1
+      simp [h1] at h2
+      grind only [PackedFloat.eq_mkZero_of_isZero']
+    · simp [hzero] at h1
+      grind only
+  · intros h
+    simp [h]
+    simp [he]
+    constructor
+    · grind
+    · intros upper hupper
+      by_cases hzero : upper.isZero
+      · simp [hzero]
+        have hupper : upper = PackedFloat.getZero e s upper.sign := by
+          grind only [PackedFloat.eq_mkZero_of_isZero']
+        rw [hupper]
+        simp [he]
+      · simp [hzero]
+        intros hsign
+        apply PackedFloat.le_of_sign_eq_true_sign_eq_false
+        · grind
+        · grind
+        · grind
+        · grind
+
+@[simp]
+theorem upper_zero_eq {eout sout : Nat} (heout : 0 < eout) :
+  (SmtLibSemantics.smtLibUpper.upper (ExtRat.Number 0) : PackedFloat eout sout) =
+    PackedFloat.getZero eout sout true := by
+  simp [SmtLibSemantics.smtLibUpper]
+  apply Classical.epsilon_elim (q := fun (x : PackedFloat eout sout) => x = PackedFloat.getZero eout sout true)
+    (y := PackedFloat.getZero eout sout true)
+  · rw [IsLawfulUpper_Zero_iff]
+    · grind
+  · intros x hx
+    simp [IsLawfulUpper_Zero_iff, heout] at hx
+    simp [hx]
+
+@[simp]
+theorem roundRTZ_zero {eout sout : Nat} {zeroSign : Bool} (heout : 0 < eout) :
+  ((SmtLibSemantics.smtLibRoundMethod eout sout SmtLibSemantics.smtLibV SmtLibSemantics.smtLibV).roundRTZ zeroSign
+    (ExtRat.Number 0)) = PackedFloat.getZero eout sout zeroSign := by
+  simp [SmtLibSemantics.RoundMethod.roundRTZ]
+  rcases zeroSign
+  case false =>
+    simp [lower_zero_eq, heout]
+  case true =>
+    simp [upper_zero_eq, heout]
+
+@[simp]
+theorem roundRNA_zero {eout sout : Nat} {zeroSign : Bool} (heout : 0 < eout) :
+  ((SmtLibSemantics.smtLibRoundMethod eout sout SmtLibSemantics.smtLibV SmtLibSemantics.smtLibV).roundRNA zeroSign
+    (ExtRat.Number 0)) = PackedFloat.getZero eout sout zeroSign := by
+  simp [SmtLibSemantics.RoundMethod.roundRNA]
+  rcases zeroSign
+  case false =>
+    simp [lower_zero_eq, heout]
+  case true =>
+    simp [upper_zero_eq, heout]
+
+@[simp]
+theorem roundRNE_zero {eout sout : Nat} {zeroSign : Bool} (heout : 0 < eout) :
+  ((SmtLibSemantics.smtLibRoundMethod eout sout SmtLibSemantics.smtLibV SmtLibSemantics.smtLibV).roundRNE zeroSign
+    (ExtRat.Number 0)) = PackedFloat.getZero eout sout zeroSign := by
+  simp [SmtLibSemantics.RoundMethod.roundRNE]
+  rcases zeroSign
+  case false =>
+    simp [lower_zero_eq, heout]
+  case true =>
+    simp [upper_zero_eq, heout]
+
+@[simp]
+theorem roundRTN_zero {eout sout : Nat} {zeroSign : Bool} (heout : 0 < eout) :
+  ((SmtLibSemantics.smtLibRoundMethod eout sout SmtLibSemantics.smtLibV SmtLibSemantics.smtLibV).roundRTN zeroSign
+    (ExtRat.Number 0)) = PackedFloat.getZero eout sout zeroSign := by
+  simp [SmtLibSemantics.RoundMethod.roundRTN]
+  rcases zeroSign
+  case false =>
+    simp [lower_zero_eq, heout]
+  case true =>
+    simp [upper_zero_eq, heout]
+
+@[simp]
+theorem roundRTP_zero {eout sout : Nat} {zeroSign : Bool} (heout : 0 < eout) :
+  ((SmtLibSemantics.smtLibRoundMethod eout sout SmtLibSemantics.smtLibV SmtLibSemantics.smtLibV).roundRTP zeroSign
+    (ExtRat.Number 0)) = PackedFloat.getZero eout sout zeroSign := by
+  simp [SmtLibSemantics.RoundMethod.roundRTP]
+  rcases zeroSign
+  case false =>
+    simp [lower_zero_eq, heout]
+  case true =>
+    simp [upper_zero_eq, heout]
+
+theorem isZero_round_zero {eout sout : Nat} {zeroSign : Bool} {rm : RoundingMode} (heout : 0 < eout) :
+  ((SmtLibSemantics.smtLibRoundMethod eout sout SmtLibSemantics.smtLibV SmtLibSemantics.smtLibV).round
+    rm zeroSign (ExtRat.Number 0)).isZero = true := by
+  rcases rm <;> simp [heout]
+
+/-- rounding a number never produces NaN. -/
+theorem isNaN_round_number_eq_false {eout sout : Nat} {zeroSign : Bool} {rm : RoundingMode} {r : Rat}
+  (heout : 0 < eout) :
+  ((SmtLibSemantics.smtLibRoundMethod eout sout SmtLibSemantics.smtLibV SmtLibSemantics.smtLibV).round
+    rm zeroSign (ExtRat.Number r)).isNaN = false := by
+  apply Classical.byContradiction
+  intros hcontra
+  simp at hcontra
+  sorry
+
+@[simp]
+theorem round_eq_mkZero_of_mkZero {zeroSign : Bool} {eout sout : Nat} {rm : RoundingMode}
+   (heout : 0 < eout) :
+    (SmtLibSemantics.smtLibRoundMethod eout sout SmtLibSemantics.smtLibV SmtLibSemantics.smtLibV).round
+        rm zeroSign (ExtRat.Number 0) = PackedFloat.getZero eout sout zeroSign := by
+  rcases rm <;> simp [heout]
+
+set_option warn.sorry false in
+
+@[simp]
+theorem IsLawfulLower_Infinity_iff (x : PackedFloat e s)
+    (he : 0 < e) (hs : 0 < s) :
+   SmtLibSemantics.IsLawfulLower (ExtRat.Infinity sign) x ↔ (x = PackedFloat.getInfinity e s sign) := by
+  simp [SmtLibSemantics.IsLawfulLower]
+  constructor
+  · intros h
+    obtain ⟨h1, h2⟩ := h
+    induction x using PackedFloat.kindCasesNaNInfZeroNum
+    case nanCase n hnan =>
+      simp [hnan] at h1
+    case infCase signx =>
+      simp [hs] at h1
+      specialize h2 (PackedFloat.getInfinity e s sign)
+      simp [hs] at h2
+      grind only [Bool]
+    case zeroCase signx =>
+      simp [he, hs] at h1
+      subst h1
+      simp at h2
+      specialize (h2 (PackedFloat.getInfinity e s false))
+      simp [hs] at h2
+      exact h2
+    case numCase n hn =>
+      specialize h2 (PackedFloat.getInfinity e s sign)
+      simp [hs] at h2
+      rw [n.toExtRat'_eq_toRat_of] at h1
+      simp at h1
+      subst h1
+      simp [hs] at h2
+      exact h2
+  · intros h
+    subst h
+    simp [hs]
+    intros lower hlower
+    rcases sign
+    case false =>
+      simp [hs] at hlower ⊢
+      grind only [=> PackedFloat.le_getInfinity_false_of_not_isNaN]
+    case true =>
+      simpa [he, hs] using hlower
+
+@[simp]
+theorem IsLawfulUpper_Infinity_iff (x : PackedFloat e s)
+    (he : 0 < e) (hs : 0 < s) :
+   SmtLibSemantics.IsLawfulUpper (ExtRat.Infinity sign) x ↔ (x = PackedFloat.getInfinity e s sign) := by
+  simp [SmtLibSemantics.IsLawfulUpper]
+  constructor
+  · intros h
+    obtain ⟨h1, h2⟩ := h
+    induction x using PackedFloat.kindCasesNaNInfZeroNum
+    case nanCase n hnan =>
+      simp only [hnan, PackedFloat.toExtRat'_eq_NaN_of_isNaN, ExtRat.ExtRat.NaN_le_iff,
+        decide_eq_true_eq, ExtRat.ExtRat.le_refl, ExtRat.ExtRat.eq_of_le_of_le,
+        ExtRat.ExtRat.le_NaN_iff, reduceCtorEq, decide_false, Bool.false_eq_true] at h1
+    case infCase signx =>
+      simp only [hs, PackedFloat.isInfinite_getInfinity, decide_true,
+        PackedFloat.toExtRat'_eq_Infinity_of_isInfinite, PackedFloat.sign_getInfinity,
+        ExtRat.ExtRat.infinity_le_infinity_iff, decide_implies, Bool.decide_eq_false, dite_eq_ite,
+        Bool.if_true_right, Bool.not_not, Bool.or_eq_true, Bool.not_eq_eq_eq_not,
+        Bool.not_true] at h1
+      specialize h2 (PackedFloat.getInfinity e s sign)
+      simp only [hs, PackedFloat.isInfinite_getInfinity, decide_true,
+        PackedFloat.toExtRat'_eq_Infinity_of_isInfinite, PackedFloat.sign_getInfinity,
+        ExtRat.ExtRat.le_refl, PackedFloat.getInfinity_le_getInfinity_iff_of_lt,
+        forall_const] at h2
+      grind only [Bool]
+    case zeroCase signx =>
+      simp only [PackedFloat.isZero_getZero, he, decide_true,
+        PackedFloat.toExtRat'_eq_zero_of_isZero, ExtRat.infinity_le_number_iff] at h1
+      subst h1
+      simp at h2
+      specialize (h2 (PackedFloat.getInfinity e s true))
+      simp only [hs, PackedFloat.isNaN_getInfinity_eq_false, decide_true, Bool.not_true,
+        PackedFloat.le_getInfinity_true_iff_eq, forall_const] at h2
+      exact h2
+    case numCase n hn =>
+      specialize h2 (PackedFloat.getInfinity e s sign)
+      simp only [hs, PackedFloat.isInfinite_getInfinity, decide_true,
+        PackedFloat.toExtRat'_eq_Infinity_of_isInfinite, PackedFloat.sign_getInfinity,
+        ExtRat.ExtRat.le_refl, forall_const] at h2
+      rw [n.toExtRat'_eq_toRat_of] at h1
+      simp at h1
+      subst h1
+      simp [hs] at h2
+      exact h2
+  · intros h
+    subst h
+    simp [hs]
+    intros upper hupper
+    rcases sign
+    case false =>
+      simp only [ExtRat.ExtRat.inf_false_le_iff, decide_eq_true_eq, hs,
+        PackedFloat.eq_getInfinity_iff_toExtRat'_eq_Infinity,
+        PackedFloat.PackedFloat.getInfinity_false_le_iff_eq] at hupper ⊢
+      grind only [=> PackedFloat.le_getInfinity_false_of_not_isNaN]
+    case true =>
+      simp only [hs, ExtRat.ExtRat.inf_true_le_iff,  ne_eq, PackedFloat.toExtRat'_eq_NaN_iff_isNaN, Bool.not_eq_true,
+        Bool.decide_eq_false, Bool.not_eq_eq_eq_not, Bool.not_true,
+        PackedFloat.PackedFloat.getInfinity_true_le_of_not_isNaN] at hupper ⊢
+      exact hupper
+
+@[simp]
+theorem lower_infinity_eq_getInfinity {e s} (sign : Bool) (he : 0 < e) (hs : 0 < s) :
+  (SmtLibSemantics.smtLibLower.lower (ExtRat.Infinity sign) : PackedFloat e s) =
+    PackedFloat.getInfinity e s sign := by
+  simp [SmtLibSemantics.smtLibLower]
+  apply Classical.epsilon_elim (q := fun (x : PackedFloat e s) => x = PackedFloat.getInfinity e s sign)
+    (y := PackedFloat.getInfinity e s sign)
+  · simp [SmtLibSemantics.IsLawfulLower, hs]
+    intros lower hlower
+    rcases sign
+    case false =>
+      simp at hlower
+      simp [hs]
+      simp [hlower]
+    case true =>
+      simp at hlower
+      simp [hs] at hlower
+      subst hlower
+      simp
+  · intros x hx
+    grind only [IsLawfulLower_Infinity_iff]
+
+@[simp]
+theorem upper_infinity_eq_getInfinity {e s} (sign : Bool) (he : 0 < e) (hs : 0 < s) :
+  (SmtLibSemantics.smtLibUpper.upper (ExtRat.Infinity sign) : PackedFloat e s) =
+    PackedFloat.getInfinity e s sign := by
+  simp [SmtLibSemantics.smtLibUpper]
+  apply Classical.epsilon_elim (q := fun (x : PackedFloat e s) => x = PackedFloat.getInfinity e s sign)
+    (y := PackedFloat.getInfinity e s sign)
+  · simp [SmtLibSemantics.IsLawfulUpper, hs]
+    intros upper hupper
+    rcases sign
+    case false =>
+      simp [hs] at hupper ⊢
+      grind only [=> PackedFloat.le_getInfinity_false_of_not_isNaN]
+    case true =>
+      simp only [hs, ExtRat.ExtRat.inf_true_le_iff, ne_eq, PackedFloat.toExtRat'_eq_NaN_iff_isNaN, Bool.not_eq_true,
+        Bool.decide_eq_false, Bool.not_eq_eq_eq_not, Bool.not_true,
+        PackedFloat.PackedFloat.getInfinity_true_le_of_not_isNaN] at hupper ⊢
+      exact hupper
+  · intros x hx
+    grind only [IsLawfulUpper_Infinity_iff]
+
+@[simp]
+theorem roundRNA_mkInfinity (eout sout : Nat) (sign : Bool) (heout : 0 < eout) (hsout : 0 < sout) :
+  ((SmtLibSemantics.smtLibRoundMethod eout sout SmtLibSemantics.smtLibV SmtLibSemantics.smtLibV).roundRNA sign
+    (ExtRat.Infinity infSign)) = (PackedFloat.getInfinity eout sout infSign) := by
+  simp [SmtLibSemantics.RoundMethod.roundRNA]
+  simp [lower_infinity_eq_getInfinity infSign heout hsout]
+  simp [SmtLibSemantics.smtLibRoundMethod.lowerHalf_eq]
+  simp [lower_infinity_eq_getInfinity infSign heout (show 0 < sout + 1 by grind)]
+  simp [heout, hsout]
+  intros ha hb
+  rcases infSign
+  · simp at ha
+  · simp at hb
+
+@[simp]
+theorem roundRNE_mkInfinity (eout sout : Nat) (sign : Bool) (heout : 0 < eout) (hsout : 0 < sout) :
+   ((SmtLibSemantics.smtLibRoundMethod eout sout SmtLibSemantics.smtLibV SmtLibSemantics.smtLibV).roundRNE sign
+    (ExtRat.Infinity infSign)) = (PackedFloat.getInfinity eout sout infSign) := by
+  simp [SmtLibSemantics.RoundMethod.roundRNE]
+  simp [lower_infinity_eq_getInfinity infSign heout hsout]
+  simp [SmtLibSemantics.smtLibRoundMethod.lowerHalf_eq]
+  simp [lower_infinity_eq_getInfinity infSign heout (show 0 < sout + 1 by grind)]
+  simp [heout, hsout]
+
+@[simp]
+theorem roundRTP_mkInfinity (eout sout : Nat) (sign : Bool) (heout : 0 < eout) (hsout : 0 < sout) :
+   ((SmtLibSemantics.smtLibRoundMethod eout sout SmtLibSemantics.smtLibV SmtLibSemantics.smtLibV).roundRTP sign
+    (ExtRat.Infinity infSign)) = (PackedFloat.getInfinity eout sout infSign) := by
+  simp [SmtLibSemantics.RoundMethod.roundRTP]
+  simp [heout, hsout]
+
+@[simp]
+theorem roundRTN_mkInfinity (eout sout : Nat) (sign : Bool) (heout : 0 < eout) (hsout : 0 < sout) :
+   ((SmtLibSemantics.smtLibRoundMethod eout sout SmtLibSemantics.smtLibV SmtLibSemantics.smtLibV).roundRTN sign
+    (ExtRat.Infinity infSign)) = (PackedFloat.getInfinity eout sout infSign) := by
+  simp [SmtLibSemantics.RoundMethod.roundRTN]
+  simp [lower_infinity_eq_getInfinity infSign heout hsout]
+
+@[simp]
+theorem roundRTZ_mkInfinity (eout sout : Nat) (sign : Bool) (heout : 0 < eout) (hsout : 0 < sout) :
+   ((SmtLibSemantics.smtLibRoundMethod eout sout SmtLibSemantics.smtLibV SmtLibSemantics.smtLibV).roundRTZ sign
+    (ExtRat.Infinity infSign)) = (PackedFloat.getInfinity eout sout infSign) := by
+  simp [SmtLibSemantics.RoundMethod.roundRTZ]
+  rcases infSign
+  case false =>
+    simp [lower_infinity_eq_getInfinity _ heout hsout]
+  case true =>
+    simp [upper_infinity_eq_getInfinity _ heout hsout]
+
+
+
+@[simp]
+theorem roundQ_eq_round_of_Infinity {zeroSign infSign : Bool} {e s : Nat} {rm : RoundingMode} (he : 0 < e ) (hs : 0 < s) :
+    (SmtLibSemantics.smtLibRoundMethod e s SmtLibSemantics.smtLibV SmtLibSemantics.smtLibV).round rm zeroSign
+      (ExtRat.Infinity infSign) =
+      PackedFloat.getInfinity e s infSign := by
+  cases rm
+  · simp [he, hs]
+  · simp [he, hs]
+  · simp [he, hs]
+  · simp [he, hs]
+  · simp [he, hs]
+
+
+end Fp
