Fp/Theorems/LowerUpperRound/Lemmas.lean
@@ -1,0 +1,38 @@
+import Fp.Theorems.LowerUpperRound.Basic
+import Fp.Theorems.LowerUpperRound.Functional
+
+namespace Fp
+
+#check PackedFloat.eq_getInfinity_of_lt_maxNormalNumber_of_isNaN_of_nonneg
+
+
+theorem lower_Number_eq_getInfinity_of_maxNormalNumber_lt
+  {ep sp : Nat}
+  (hep : 0 < ep)
+  (hsp : 0 < sp)
+  (r : Rat)
+  (hx :  r < (PackedFloat.maxNormalNumber ep sp true).toRat) :
+  lower ep sp hep hsp (ExtRat.Number r) = PackedFloat.getInfinity ep sp false := by
+  rw [lower]
+  simp
+  have : r ≠ 0 := by sorry
+  simp [this]
+  sorry
+
+
+theorem upper_Number_eq_getInfinity_of_maxNormalNumber_lt
+  {ep sp : Nat}
+  (hep : 0 < ep)
+  (hsp : 0 < sp)
+  (r : Rat)
+  (hx : (PackedFloat.maxNormalNumber ep sp false).toRat < r) :
+  upper ep sp hep hsp (ExtRat.Number r) = PackedFloat.getInfinity ep sp false := by
+  rw [upper]
+  simp only [ExtRat.ExtRat.neg_number]
+  rw [lower]
+  simp
+  have : r ≠ 0 := by sorry
+  simp [this]
+  sorry
+
+end Fp
