Fp/Theorems/PackedUnpackedRel/Basic.lean
@@ -1,0 +1,61 @@
+import Fp.PackedFloat.Basic
+import Fp.UnpackedFloat.Basic
+import Fp.Theorems.UnpackedFloat.ToRat
+import Fp.EUnpackedFloat.Basic
+import Fp.Basic
+
+
+/--
+An unpacked float is related to a packed float
+iff they have the same rational value and the same sign.
+-/
+def UnpackedFloat.Rel (uf : UnpackedFloat e s) (pf : PackedFloat ep sp) :=
+  uf.toRat' = pf.toRat ∧ uf.sign = pf.sign -- ∧ ¬ pf.isInfinite ∧ ¬ pf.isNaN
+
+
+@[grind =>]
+theorem UnpackedFloat.Rel_of_toRat_eq_toRat_and_sign (uf : UnpackedFloat ef uf) (pf : PackedFloat ep sp)
+  (hToRat : uf.toRat' = pf.toRat) (hSign : uf.sign = pf.sign) :
+  UnpackedFloat.Rel uf pf := by
+  simp only [UnpackedFloat.Rel]
+  simp [hToRat, hSign]
+
+theorem UnpackedFloat.Rel_of_isZero_of_isZero
+  (uf : UnpackedFloat ef uf)
+  (pf : PackedFloat ep sp)
+  (huf : uf.isZero) (hpf : pf.isZero) (hsign : uf.sign = pf.sign) :
+  UnpackedFloat.Rel uf pf := by
+  simp only [UnpackedFloat.Rel]
+  simp [hpf, hsign, huf]
+
+/--
+An extended unpacked float is related to a packed float
+iff they are both NaN, or they are both infinite with the same sign,
+or they are either NaN and infinite, and have the same rational value and the same sign.
+-/
+def EUnpackedFloat.Rel (euf : EUnpackedFloat ef uf) (pf : PackedFloat ep sp) :=
+  (euf.isNaN ∧ pf.isNaN) ∨
+  (euf.isInfinite ∧ pf.isInfinite ∧ euf.sign = pf.sign) ∨
+  (¬ euf.isNaN ∧ ¬ euf.isInfinite ∧ euf.num.Rel pf)
+
+@[simp, grind =>]
+theorem EUnpackedFloat.Rel_of_isNaN_of_isNaN (euf : EUnpackedFloat ef uf)
+  (pf : PackedFloat ep sp)
+  (heuf : euf.isNaN) (hpf : pf.isNaN) :
+  EUnpackedFloat.Rel euf pf := by
+  simp only [EUnpackedFloat.Rel]
+  simp [heuf, hpf]
+
+@[simp, grind =>]
+theorem EUnpackedFloat.Rel_of_isInfinite_of_isInfinite_and_sign (euf : EUnpackedFloat ef uf) (pf : PackedFloat ep sp)
+  (heuf : euf.isInfinite) (hpf : pf.isInfinite) (hsign : euf.sign = pf.sign) :
+  EUnpackedFloat.Rel euf pf := by
+  simp only [EUnpackedFloat.Rel]
+  simp [heuf, hpf, hsign]
+
+@[simp, grind =>]
+theorem EUnpackedFloat.Rel_of_Rel_of_not_isNaN_of_not_isInfinite (euf : EUnpackedFloat ef uf) (pf : PackedFloat ep sp)
+  (heuf : ¬ euf.isNaN) (heuf' : ¬ euf.isInfinite) (hRel : euf.num.Rel pf) :
+  EUnpackedFloat.Rel euf pf := by
+  simp only [EUnpackedFloat.Rel]
+  simp [heuf, heuf', hRel]
